try to introduce a table

src/tls/Crypto.AEAD.fst
@@ -11,14 +11,59 @@ module HS = FStar.HyperStack
 module HST = FStar.HyperStack.ST
 module EE = EverCrypt.Error
 module G = FStar.Ghost
+module MDM = FStar.Monotonic.DependentMap
 
-type plain_pred = (plain: Seq.seq U8.t) -> Tot Type0
+type plain_pred = (plain: Seq.seq SC.uint8) -> Tot Type0
+
+// inline_for_extraction
+let ideal: bool = false
+
+noextract
+inline_for_extraction
+let entry (a: SC.supported_alg): Tot eqtype =
+  [@inline_let]
+  let t = SC.iv a & SC.cipher a in
+  assume (hasEq t);
+  t
 
 inline_for_extraction
-type state (a: SC.supported_alg) (phi: plain_pred) = (s: B.pointer (EC.state_s a))
+let table
+  (a: SC.supported_alg)
+  (kv: SC.kv a)
+  (phi: plain_pred)
+: Tot Type0
+= MDM.t HS.root (entry a) (fun (iv, cipher) -> (plain: SC.plain a { phi plain /\ SC.encrypt kv iv Seq.empty plain == cipher })) (fun _ -> True)
+
+inline_for_extraction
+noeq
+type state (a: SC.supported_alg) (phi: plain_pred) = {
+  ec: B.pointer (EC.state_s a);
+  kv: Ghost.erased (SC.kv a);
+  table: (if ideal then table a (Ghost.reveal kv) phi else unit)
+}
 
 let invariant (#a: SC.supported_alg) (#phi: plain_pred) (h: HS.mem) (s: state a phi) : GTot Type0 =
-  EC.invariant h s
+  EC.invariant h s.ec /\
+  EC.as_kv (B.deref h s.ec) == G.reveal s.kv /\
+  (
+    if ideal
+    then B.loc_disjoint (EC.footprint h s.ec) (B.loc_mreference (s.table <: table a (G.reveal s.kv) phi)) /\ h `HS.contains` (s.table <: table a (G.reveal s.kv) phi)
+    else True
+  )
+
+let footprint (#a: SC.supported_alg) (#phi: plain_pred) (h: HS.mem) (s: state a phi) : GTot B.loc =
+  EC.footprint h s.ec `B.loc_union` (if ideal then B.loc_mreference (s.table <: table a (G.reveal s.kv) phi) else B.loc_none)
+
+let encrypted (#a: SC.supported_alg) (#phi: plain_pred) (s: state a phi) (cipher: SC.cipher a) : GTot Type0 =
+  if ideal
+  then
+    Seq.length cipher >= 12 + SC.tag_length a /\ (
+    let iv = Seq.slice cipher 0 12 in
+    let cipher' = Seq.slice cipher 12 (Seq.length cipher) in
+    HST.witnessed (MDM.defined (s.table <: table a (G.reveal s.kv) phi) (iv, cipher'))
+  )
+  else
+    True
 
 noextract
 inline_for_extraction
@@ -45,8 +90,9 @@ let encrypt
     invariant h s /\
     B.live h plain /\
     B.live h cipher /\
-    B.loc_disjoint (EC.footprint h s) (B.loc_buffer plain) /\
-    B.loc_disjoint (EC.footprint h s) (B.loc_buffer cipher) /\
+    phi (B.as_seq h plain) /\
+    B.loc_disjoint (footprint h s) (B.loc_buffer plain) /\
+    B.loc_disjoint (footprint h s) (B.loc_buffer cipher) /\
     B.disjoint plain cipher /\
     B.length cipher == B.length plain + 12 + SC.tag_length a
   ))
@@ -55,8 +101,8 @@ let encrypt
     | EE.InvalidKey ->
       B.modifies B.loc_none h h'
     | EE.Success ->
-      EC.footprint h' s == EC.footprint h s /\
-      B.modifies (B.loc_union (EC.footprint h s) (B.loc_buffer cipher)) h h' /\
+      footprint h' s == footprint h s /\
+      B.modifies (B.loc_union (footprint h s) (B.loc_buffer cipher)) h h' /\
       invariant h' s
     | _ -> False
   ))
@@ -67,9 +113,9 @@ let encrypt
   let ad_len = 0ul in
   let cipher' = B.sub cipher iv_len plain_len in
   let tag' = B.sub cipher (iv_len `U32.add` plain_len) (tag_len a) in
-  EC.encrypt
+  let res = EC.encrypt
     #(G.hide a)
-    s
+    s.ec
     iv
     iv_len
     ad
@@ -78,6 +124,10 @@ let encrypt
     plain_len
     cipher'
     tag'
+  in
+  let h' = HST.get () in
+  assume (EC.as_kv (B.deref h' s.ec) == G.reveal s.kv);
+  res
 
 let decrypt
   (#a: SC.supported_alg)
@@ -92,8 +142,8 @@ let decrypt
     B.live h plain /\
     B.live h cipher /\
     B.length cipher == B.length plain + 12 + SC.tag_length a /\
-    B.loc_disjoint (EC.footprint h s) (B.loc_buffer plain) /\
-    B.loc_disjoint (EC.footprint h s) (B.loc_buffer cipher) /\
+    B.loc_disjoint (footprint h s) (B.loc_buffer plain) /\
+    B.loc_disjoint (footprint h s) (B.loc_buffer cipher) /\
     B.disjoint plain cipher
   ))
   (ensures (fun h res h' ->
@@ -102,8 +152,8 @@ let decrypt
       B.modifies B.loc_none h h'
     | EE.Success
     | EE.AuthenticationFailure ->
-      B.modifies (B.loc_union (EC.footprint h s) (B.loc_buffer plain)) h h' /\
-      EC.footprint h' s == EC.footprint h s /\
+      B.modifies (B.loc_union (footprint h s) (B.loc_buffer plain)) h h' /\
+      footprint h' s == footprint h s /\
       invariant h' s
     | _ -> False
   ))
@@ -114,9 +164,9 @@ let decrypt
   let plain_len = cipher_len `U32.sub` tag_len a `U32.sub` iv_len in
   let cipher' = B.sub cipher iv_len plain_len in
   let tag' = B.sub cipher (iv_len `U32.add` plain_len) (tag_len a) in
-  EverCrypt.AEAD.decrypt
+  let res = EverCrypt.AEAD.decrypt
     #(G.hide a)
-    s
+    s.ec
     iv
     iv_len
     ad
@@ -125,4 +175,7 @@ let decrypt
     plain_len
     tag'
     plain
-
+  in
+  let h' = HST.get () in
+  assume (EC.as_kv (B.deref h' s.ec) == G.reveal s.kv);
+  res
